Main.lean
@@ -1,7 +1,6 @@
 import BlockSynchroniser
 import BlockSynchroniser.Definitions
 
-open BlockSynchroniser.Examples
 
 def main : IO Unit :=
-  IO.println s!"Hello, BlockSynchroniser! System has {exampleSystem.n} validators."
+  IO.println s!"Hello, BlockSynchroniser! System has X validators."
